Simplify PCM2 some more

Test/modules/PCM2.dfy
@@ -1,29 +1,11 @@
-module GhostLoc {
-  datatype Loc =
-    | BaseLoc(ghost t: nat)
-    | ExtLoc(ghost s: nat, ghost base_loc: Loc)
-}
 abstract module PCM {
-  import opened GhostLoc
   type M(!new)
-  predicate transition(a: M, b: M)
   least predicate reachable(a: M, b: M) {
-    a == b || (exists z :: reachable(a, z) && transition(z, b))
+    a == b || (exists z :: reachable(a, z))
   }
 }
-module Tokens(pcm: PCM) {
-  import opened GhostLoc
-  type {:extern} Token(!new)
-  function {:extern} loc(t:Token) : Loc
-  function {:extern} get(t:Token) : pcm.M
-}
 abstract module PCMExt(Base: PCM) refines PCM {
-  type B = Base.M
-  type F = M
 }
 module PCMExtMethods(Base: PCM, Ext: PCMExt(Base)) {
   type B = Base.M
-  type F = Ext.M
-  import BaseTokens = Tokens(Base)
-  import ExtTokens = Tokens(Ext)
 }
